src/3d/prelude/Prelude.fsti
@@ -1,0 +1,201 @@
+(*
+   Copyright 2019 Microsoft Research
+
+   Licensed under the Apache License, Version 2.0 (the "License");
+   you may not use this file except in compliance with the License.
+   You may obtain a copy of the License at
+
+       http://www.apache.org/licenses/LICENSE-2.0
+
+   Unless required by applicable law or agreed to in writing, software
+   distributed under the License is distributed on an "AS IS" BASIS,
+   WITHOUT WARRANTIES OR CONDITIONS OF ANY KIND, either express or implied.
+   See the License for the specific language governing permissions and
+   limitations under the License.
+*)
+module Prelude
+include Prelude.StaticHeader
+include ResultOps
+module U32 = FStar.UInt32
+module U16 = FStar.UInt16
+module U64 = FStar.UInt64
+
+////////////////////////////////////////////////////////////////////////////////
+// Parsers
+////////////////////////////////////////////////////////////////////////////////
+
+inline_for_extraction
+noextract
+val parser_kind (nz:bool) : Type0
+
+inline_for_extraction
+noextract
+val parser (#nz:bool) (k:parser_kind nz) (t:Type0) : Type0
+
+inline_for_extraction
+noextract
+val glb (#nz1:bool) (k1:parser_kind nz1)
+        (#nz2:bool) (k2:parser_kind nz2)
+    : parser_kind (nz1 && nz2)
+
+/// Parser: return
+inline_for_extraction
+noextract
+val ret_kind : parser_kind false
+
+inline_for_extraction noextract
+val parse_ret (#t:Type) (v:t)
+  : Tot (parser ret_kind t)
+
+/// Parser: bind
+inline_for_extraction
+noextract
+val and_then_kind (#nz1:_) (k1:parser_kind nz1)
+                  (#nz2:_) (k2:parser_kind nz2)
+    : parser_kind (nz1 || nz2)
+
+inline_for_extraction noextract
+val parse_dep_pair (#nz1:_) (#k1:parser_kind nz1) (#t1: Type0) (p1: parser k1 t1)
+                   (#nz2:_) (#k2:parser_kind nz2) (#t2: (t1 -> Tot Type0)) (p2: (x: t1) -> parser k2 (t2 x))
+  : Tot (parser (and_then_kind k1 k2) (dtuple2 t1 t2) )
+
+/// Parser: sequencing
+inline_for_extraction noextract
+val parse_pair (#nz1:_) (#k1:parser_kind nz1) (#t1:_) (p1:parser k1 t1)
+               (#nz2:_) (#k2:parser_kind nz2) (#t2:_) (p2:parser k2 t2)
+  : Tot (parser (and_then_kind k1 k2) (t1 * t2))
+
+/// Parser: filter
+let refine t (f:t -> bool) = x:t{f x}
+
+inline_for_extraction
+noextract
+val filter_kind (#nz:_) (k:parser_kind nz) : parser_kind nz
+
+inline_for_extraction noextract
+val parse_filter (#nz:_) (#k:parser_kind nz) (#t:_) (p:parser k t) (f:(t -> bool))
+  : Tot (parser (filter_kind k) (refine t f))
+
+
+inline_for_extraction noextract
+val parse_weaken_left (#nz:_)  (#k:parser_kind nz) (#t:_) (p:parser k t)
+                      (#nz':_) (k':parser_kind nz')
+  : Tot (parser (glb k' k) t)
+
+inline_for_extraction noextract
+val parse_weaken_right (#nz:_)  (#k:parser_kind nz) (#t:_) (p:parser k t)
+                       (#nz':_) (k':parser_kind nz')
+  : Tot (parser (glb k k') t)
+
+inline_for_extraction
+noextract
+val impos_kind : parser_kind true
+
+/// Parser: unreachable, for default cases of exhaustive pattern matching
+inline_for_extraction noextract
+val parse_impos (_:unit)
+  : parser impos_kind False
+
+let t_ite (e:bool) (a:Type) (b:Type) = if e then a else b
+
+val parse_ite (#nz:_) (#k:parser_kind nz) (#a:Type) (#b:Type) (e:bool)
+              (p1:squash e -> parser k a)
+              (p2:squash (not e) -> parser k b)
+  : Tot (parser k (t_ite e a b))
+
+////////////////////////////////////////////////////////////////////////////////
+// Variable-sized list whose size in bytes is exactly n
+////////////////////////////////////////////////////////////////////////////////
+val nlist (n:U32.t) (t:Type0) : Type0
+
+/// Lists/arrays
+inline_for_extraction
+noextract
+val kind_nlist : parser_kind false
+
+inline_for_extraction noextract
+val parse_nlist (n:U32.t) (#k:parser_kind true) (#t:_) (p:parser k t)
+  : Tot (parser kind_nlist (nlist n t))
+
+
+////////////////////////////////////////////////////////////////////////////////
+// Variable-sized element whose size in bytes is at most n
+////////////////////////////////////////////////////////////////////////////////
+val t_at_most (n:U32.t) (t:Type0) : Type0
+
+/// Lists/arrays
+inline_for_extraction
+noextract
+val kind_t_at_most : parser_kind false
+
+inline_for_extraction noextract
+val parse_t_at_most (n:U32.t) (#k:parser_kind true) (#t:_) (p:parser k t)
+  : Tot (parser kind_t_at_most (t_at_most n t))
+
+////////////////////////////////////////////////////////////////////////////////
+// Readers
+////////////////////////////////////////////////////////////////////////////////
+
+inline_for_extraction noextract
+val reader (#nz:_) (#k:parser_kind nz) (#t:_) (p:parser k t) : Type u#1
+
+inline_for_extraction noextract
+val read_filter (#nz:_)
+                (#k: parser_kind nz)
+                (#t: Type0)
+                (#p: parser k t)
+                (p32: reader p)
+                (f: (t -> bool))
+    : reader (parse_filter p f)
+
+////////////////////////////////////////////////////////////////////////////////
+// Base types
+////////////////////////////////////////////////////////////////////////////////
+
+
+/// UINT8
+let ___UINT8 : eqtype = FStar.UInt8.t
+inline_for_extraction noextract
+val kind____UINT8 : parser_kind true
+val parse____UINT8 : parser kind____UINT8 ___UINT8
+val read____UINT8 : reader parse____UINT8
+
+/// UInt16
+let ___UINT16 : eqtype = U16.t
+inline_for_extraction noextract
+val kind____UINT16 : parser_kind true
+val parse____UINT16 : parser kind____UINT16 ___UINT16
+val read____UINT16 : reader parse____UINT16
+
+/// UInt32
+let ___UINT32 : eqtype = U32.t
+inline_for_extraction noextract
+val kind____UINT32 : parser_kind true
+val parse____UINT32 : parser kind____UINT32 ___UINT32
+val read____UINT32 : reader parse____UINT32
+
+/// UInt64
+let ___UINT64 : eqtype = U64.t
+inline_for_extraction noextract
+val kind____UINT64 : parser_kind true
+val parse____UINT64 : parser kind____UINT64 ___UINT64
+val read____UINT64 : reader parse____UINT64
+
+inline_for_extraction noextract
+let kind_unit : parser_kind false = ret_kind
+let parse_unit : parser kind_unit unit = parse_ret ()
+inline_for_extraction noextract
+val read_unit
+  : reader (parse_ret ())
+
+////////////////////////////////////////////////////////////////////////////////
+//Convenience lemmas for bounded arithmetic, especially on bitfields
+////////////////////////////////////////////////////////////////////////////////
+
+let max_int_sizes
+  : squash FStar.UInt.(
+      max_int 10 == 1023 /\
+      max_int 8 == 255
+    )
+  = let open FStar.UInt in
+    normalize_term_spec (max_int 10)
